WIP trace proofs

aneris/examples/transactional_consistency/read_uncommitted/trace/implication_trace.v
@@ -9,35 +9,71 @@ From aneris.aneris_lang.lib.serialization Require Import serialization_proof.
 From aneris.aneris_lang.program_logic Require Import lightweight_atomic.
 From aneris.examples.transactional_consistency Require Import code_api wrapped_library.
 From aneris.examples.transactional_consistency.read_uncommitted.specs Require Import specs resources.
-From aneris.examples.transactional_consistency Require Import user_params aux_defs state_based_model.
+From aneris.examples.transactional_consistency Require Import resource_algebras user_params aux_defs state_based_model.
 
 Section trace_proof.
-  Context `{!anerisG Mdl Σ, !User_params}.
+  Context `{!anerisG Mdl Σ, !KVSG Σ, !User_params}.
 
   Definition trace_inv_name := nroot.@"trinv".
 
-  (** Ghost theory *)
+  (** Ghost theory for wrapped resources *)
+
+  Definition OwnLinTrace (γ : gname) (l : list val) : iProp Σ := True.
+
+  Definition OwnLinHist (γ : gname) (l : list val) : iProp Σ := True.
+
+  Lemma own_lin_hist (γ : gname) (l h : list val) :
+    OwnLinTrace γ l ==∗ OwnLinTrace γ l ∗ OwnLinHist γ h.
+  Proof.
+  Admitted.
+
+  Lemma own_lin_prefix (γ : gname) (l h : list val) :
+    OwnLinTrace γ l -∗ 
+    OwnLinHist γ h -∗
+    (OwnLinTrace γ l ∗ OwnLinHist γ h ∗ ⌜h `prefix_of` l⌝).
+  Proof.
+  Admitted.
+
+  Definition OwnTok (γ : gname) : iProp Σ := own γ (Excl ()).
+
+  Lemma own_tok_excl (γ : gname) : 
+    OwnTok γ -∗ OwnTok γ -∗ False.
+  Proof. 
+    iIntros "H1 H2". 
+    by iDestruct (own_valid_2 with "H1 H2") as %?.
+  Qed.
+
+  (** Predicates for wrapped resources *)
+
+  Definition last_commit : Prop := true.
+
+  Definition open_start : Prop := true. 
+
+  Definition latest_write : Prop := true. 
 
   (** Wrapped resources  *)
-  (* Global Program Instance wrapped_resources `(res : !RU_resources Mdl Σ) : RU_resources Mdl Σ :=
+  (* Global Program Instance wrapped_resources (γm1 γm2 γl : gname) `(res : !RU_resources Mdl Σ) : RU_resources Mdl Σ :=
     {|
-      GlobalInv := (GlobalInv ∗ trace_inv trace_inv_name valid_trace_ru ∗ ∃ t, trace_is t ∗
-                   (∀ c, ⌜latest c t_hist t⌝ ∗ OwnHalfLatest c t_hist))%I;
-      OwnMemKey k V := (OwnMemKey k V 
-                        ∗ (∀ v, ⌜v ∈ V⌝ → ∃ t tag c, trace_hist t ∗ 
-                                ⌜(#(LitString tag), (c, (#"Wr", (#(LitString k), v))))%V ∈ t⌝))%I;
-      OwnLocalKey k c vo := (∃ t, OwnLocalKey k c vo ∗ (∀ v, ⌜vo = Some v⌝ → OwnHalfWrite k vo))%I;
-      ConnectionState c s sa := (ConnectionState c s sa ∗ 
-                                 (∃ t i, trace_hist t_hist ∗ OwnHalfLatest c t_hist ∗
-                                         (⌜s = CanStart⌝ ∗ 
-                                          (⌜is_cm_post_event (last t_hist)⌝ ∨ ⌜is_st_pre_event (last t_hist)⌝)) ∨ 
-                                         (⌜s = (Active dom)⌝ ∗ 
-                                          (∃) ∗
-                                          (∀ k, ⌜latest_write k vo t_hist⌝ ∗ OwnHalfWrite k vo))))%I;
+      GlobalInv := (GlobalInv ∗ trace_inv trace_inv_name valid_trace_ru ∗ 
+                    ∃ t lt T, trace_is t ∗ OwnLinTrace γl lt ∗ ⌜lin_trace_of lt t⌝ ∗ ⌜extraction_of lin_trace T⌝ ∗
+                      (∃ (m : gmap socket_address local_state), ghost_map_auth γm1 (1%Qp) m ∗ 
+                        (∀ sa s, m !! sa = Some s → 
+                          (((⌜s = CanStart⌝ ∗ (∃ e, ⌜last_commit c e lt⌝) ∗
+                             ∀ k, ⌜k ∈ KVS_keys⌝ → OwnWriteHalf c k ov ∗ OwnWriteHalf c k ov) ∨ 
+                            (⌜s = Active domain⌝ ∗ (∃ e, ⌜open_start c e lt⌝) ∗
+                             (∀ k, ⌜k ∈ domain⌝ → ∃ ov, OwnWriteHalf c k ov ∗ ⌜latest_write c k ov⌝) ∗
+                             (∀ k, ⌜k ∈ KVS_keys / domain⌝ → OwnWriteHalf c k ov ∗ OwnWriteHalf c k ov)))))) ∗
+                      (∃ (m : gmap string gname), ⌜∀ x, x ∈ dom m ↔ x ∈ tags t⌝ ∗ ghost_map_auth γm2 (1%Qp) m ∗
+                        (∀ e_pre tag, ⌜e_pre ∈ t⌝ → ⌜is_pre_event e_pre⌝ → ⌜tagOfEvent e_pre = Some tag⌝ →
+                          (∃ e_lin, ⌜e_lin ∈ lt⌝ ∧ ⌜tag_eq e_pre e_lin⌝) → ∃ γ, m !! tag = Some γ ∗ OwnTok γ)))%I;
+      OwnMemKey k V := (OwnMemKey k V  ∗ (∀ v, ⌜v ∈ V⌝ → ∃ lt tag c, OwnLinHist t ∗ 
+                        ⌜(#(LitString tag), (c, (#"WrLin", (#(LitString k), v))))%V ∈ t⌝))%I;
+      OwnLocalKey k c ov := (OwnLocalKey k c ov ∗ OwnWriteHalf c k ov)%I;
+      ConnectionState c s sa := (ConnectionState c s sa ∗ ghost_map_elem γm1 sa (1%Qp) s)%I; 
       IsConnected c sa := IsConnected c sa%I;
       KVS_ru := KVS_ru;
       KVS_Init := KVS_Init%I;
-      KVS_ClientCanConnect sa := KVS_ClientCanConnect sa%I;
+      KVS_ClientCanConnect sa := KVS_ClientCanConnect sa ∗ ghost_map_elem γm1 sa CanStart%I;
       Seen k V := Seen k V%I;
     |}.
   Next Obligation.
@@ -58,5 +94,7 @@ Section trace_proof.
   Proof.
     iIntros "([%res (Hkeys & Hkvs_init & Hglob_inv & Hcan_conn & 
       (#Hinit_kvs & #Hinit_cli & #Hread & #Hwrite & #Hstart & #Hcom))] & Htr & #Htr_inv)".
+  iModIntro.
+  iExists _.
   Admitted.
 End trace_proof.
